theories/IterativeEquations.v
@@ -1,0 +1,197 @@
+Require Import CSL.IterativeContract.
+Require Import Setoid.
+Require Import Init.Tauto btauto.Btauto.
+Require Import Bool.Bool.
+Require Import Lists.List.
+Import ListNotations.
+(*******************************************************************************************************)
+
+
+Definition contract_relation := Contract -> Contract -> Prop.
+
+Notation "c0 ==~== c1" := (forall s, s ==~ c0 <-> s ==~ c1) (at level 73, no associativity).
+
+Definition non_empty_relation (R : contract_relation) := exists c0 c1, R c0 c1.
+
+Definition bisimulation (R: contract_relation) := non_empty_relation R /\ forall c0 c1, R c0 c1 -> nu c0 = nu c1 /\ forall e, R (c0/e) (c1/e).
+
+(*c0 and c1 are in a bisimilarity written as c0 ~ c1*)
+Notation "c0 ~ c1" := (exists R, bisimulation R /\ R c0 c1)(at level 73, no associativity).
+
+(*
+Lemma bi_union : forall R0 R1, bisimulation R0 -> bisimulation R1 -> bisimulation (fun x y => R0 x y \/ R1 x y).
+Proof.
+intros. destruct H, H0. destruct H0 as [c0 [c1 P]]. split.
+- exists c0. exists c1. right. auto.
+- intros. destruct H0.
+  * apply H1 in H0 as [H0 H0']. split ; auto.
+  * apply H2 in H0 as [H0 H0']. split ; auto.
+Qed.*)
+
+Lemma simpl_bisim_nu : forall (c0 c1 : Contract), c0 ~ c1 -> nu c0 = nu c1.
+Proof. 
+intros. destruct H. destruct H. unfold bisimulation in H.
+destruct H. specialize H1 with c0 c1.
+apply H1 in H0. destruct H0. assumption. 
+Qed.
+
+Lemma simpl_bisim_derive : forall (c0 c1 : Contract)(e : EventType), 
+                           c0 ~ c1 -> c0/e ~ c1/e.
+Proof. intros.  destruct H. exists x. destruct H. split;auto.
+       destruct H. apply H1 in H0. destruct H0. auto.
+Qed.
+
+Hint Resolve simpl_bisim_nu  simpl_bisim_derive : bisimB.
+
+CoInductive Bisimilarity : Contract -> Contract -> Prop :=
+ CBisimilarity c0 c1 (H0: forall e, Bisimilarity (c0/e) (c1/e)) (H1: nu c0 = nu c1) : Bisimilarity c0 c1.
+
+(*Bisimilarity predicate over contract relations*)
+Definition bisimilarity (R : contract_relation) := forall c0 c1, R c0 c1 <-> Bisimilarity c0 c1.
+Global Transparent bisimilarity.
+
+Lemma exists_bisimulation_i_Bisimilarity : forall c0 c1, c0 ~ c1 -> Bisimilarity c0 c1.
+Proof.
+cofix exists_bisimulation_i_Bisimilarity.
+intros. constructor.
+- intros. apply exists_bisimulation_i_Bisimilarity. auto with bisimB.
+- auto with bisimB.
+Qed.
+
+Lemma Bisimilarity_is_bisimulation : bisimulation Bisimilarity.
+Proof.
+split;intros.
+- exists Failure. exists Failure. cofix Bisimilarity_is_bisimulation.
+  apply CBisimilarity;intros;simpl;auto.
+- destruct H; split;auto.
+Qed.
+
+Lemma Bisimilarity_i_exists_bisimulation : forall c0 c1, Bisimilarity c0 c1 -> c0 ~ c1.
+Proof.
+intros. exists Bisimilarity. split;auto using Bisimilarity_is_bisimulation.
+Qed. 
+
+(*Sanity check*)
+Theorem exists_bisimulation_is_bisimilarity : bisimilarity (fun c0 c1 => c0 ~ c1). 
+Proof.
+split; auto using exists_bisimulation_i_Bisimilarity,Bisimilarity_i_exists_bisimulation.
+Qed.
+
+
+Lemma bisimilarity_non_empty : forall (R : contract_relation), bisimilarity R -> non_empty_relation R.
+Proof.
+intros. destruct H with Failure Failure.
+assert (HA: Bisimilarity Failure Failure).
+{ cofix bisimilarity_non_empty. constructor. intros. now simpl. auto.  }
+exists Failure. exists Failure. auto.
+Qed.
+ 
+Lemma bisimilarity_i_bisimulation : forall (R : contract_relation), bisimilarity R -> bisimulation R.
+Proof.
+intros. unfold bisimilarity in H. split;auto using bisimilarity_non_empty.
+intros. pose proof H. destruct H with c0 c1. apply H1 in H0.
+destruct H0. split;auto. intros. rewrite H1. auto.
+Qed.
+
+
+Lemma matches_eq_is_bisimulation : bisimulation (fun c0 c1 => c0 ==~== c1).
+Proof.
+split.
+- exists Failure. exists Failure. reflexivity.
+- split.
+  * apply eq_true_iff_eq. now repeat rewrite nu_empty.
+  * intros. now repeat rewrite <- derive_spec_comp. 
+Qed.
+
+(*c0 ==~== c1 is a bisimilarity*)
+Theorem matches_eq_is_bisimilarity : bisimilarity (fun c0 c1 => forall s, s ==~ c0 <-> s ==~ c1).
+Proof.
+split. 
+- generalize dependent c1. generalize dependent c0. cofix matches_eq_is_bisimilarity.
+  intros. constructor.
+  * intros. apply matches_eq_is_bisimilarity. setoid_rewrite <- derive_spec_comp. auto.
+  * apply eq_true_iff_eq. repeat rewrite nu_empty. auto.
+- intro.
+  repeat setoid_rewrite matches_Matches. intro. generalize dependent c1.
+  generalize dependent c0. induction s;intros.
+  * inversion H. repeat rewrite <- matches_Matches. repeat rewrite <- nu_empty.
+    now rewrite H1.
+  * repeat rewrite derive_spec2. inversion H. auto.
+Qed.
+
+
+
+
+
+Reserved Notation "c0 =R= c1" (at level 63).
+
+CoInductive c_eq : Contract -> Contract -> Prop :=
+  | c_plus_assoc c0 c1 c2 : (c0 _+_ c1) _+_ c2 =R= c0 _+_ (c1 _+_ c2)
+  | c_plus_comm c0 c1: c0 _+_ c1 =R= c1 _+_ c0
+  | c_plus_neut c: c _+_ Failure =R= c
+  | c_plus_idemp c : c _+_ c =R= c 
+  | c_seq_assoc c0 c1 c2 : (c0 _;_ c1) _;_ c2 =R= c0 _;_ (c1 _;_ c2)
+  | c_seq_neut_l c : (Success _;_ c) =R= c 
+  | c_seq_neut_r c : c _;_ Success =R= c 
+  | c_seq_failure_l c : Failure _;_ c =R= Failure    (*EXTRA AXIOM*)
+  | c_seq_failure_r c :  c _;_ Failure =R= Failure 
+  | c_distr_l c0 c1 c2 : c0 _;_ (c1 _+_ c2) =R= (c0 _;_ c1) _+_ (c0 _;_ c2)
+  | c_distr_r c0 c1 c2 : (c0 _+_ c1) _;_ c2 =R= (c0 _;_ c2) _+_ (c1 _;_ c2)
+  | c_refl c : c =R= c
+  | c_sym c0 c1 (H: c0 =R= c1) : c1 =R= c0
+  | c_trans c0 c1 c2 (H1 : c0 =R= c1) (H2 : c1 =R= c2) : c0 =R= c2
+  | c_plus_morph c0 c0' c1 c1' (H1 : c0 =R= c0') (H2 : c1 =R= c1') : c0 _+_ c1 =R= c0' _+_ c1'
+  | c_seq_morph c0 c0' c1 c1' (H1 : c0 =R= c0') (H2 : c1 =R= c1') : c0 _;_ c1 =R= c0' _;_ c1'
+  | c_fold_unfold c : Star c =R= Success _+_ (c _;_ Star c)
+  where "c1 =R= c2" := (c_eq c1 c2).
+
+Hint Constructors c_eq : core.
+
+Add Parametric Relation : Contract c_eq
+  reflexivity proved by c_refl
+  symmetry proved by c_sym
+  transitivity proved by c_trans
+  as Contract_setoid.
+
+Add Parametric Morphism : CPlus with
+signature c_eq ==> c_eq ==> c_eq as c_eq_plus_morphism.
+Proof.
+  intros. auto.
+Qed.
+
+Add Parametric Morphism : CSeq with
+signature c_eq ==> c_eq ==> c_eq as c_eq_seq_morphism.
+Proof.
+  intros. auto.
+Qed.
+
+Lemma c_eq_is_bisimilarity : bisimilarity c_eq.
+Proof. Admitted.
+
+
+Ltac rewrite_to_Bisimilarity H0 H1 := pose proof H0; unfold bisimilarity in H0;rewrite H0 in H1;clear H0.
+
+Theorem c_eq_soundness : forall c0 c1, c0 =R= c1 -> c0 ==~== c1.
+Proof.
+intros. pose proof c_eq_is_bisimilarity. pose proof matches_eq_is_bisimilarity.
+unfold bisimilarity in *. specialize H1 with c0 c1.
+apply <- H1. now apply H0.
+Qed.
+
+Theorem c_eq_completeness : forall c0 c1, c0 ==~== c1 -> c0 =R= c1.
+Proof.
+intros. pose proof c_eq_is_bisimilarity. pose proof matches_eq_is_bisimilarity.
+unfold bisimilarity in *. rewrite H0. now rewrite <- H1.
+Qed.
+
+
+(*Possibly useful lemmas to rewrite without using the rewrite tactic*)
+Lemma rewrite_left : forall c0 c1 c2,c1 =R= c0 -> c0 =R= c2-> c1 =R= c2.
+Proof.
+intros. eauto.
+Qed.
+
+Lemma rewrite_right : forall c0 c1 c2, c2 =R= c0 -> c1 =R= c0-> c1 =R= c2.
+Proof.
+intros. eauto.
+Qed.
